Append relir

theories/RelIR.v
@@ -63,3 +63,53 @@ Proof.
       apply IHexecute2. apply IHa2. apply IHa1. reflexivity.
     + apply ER_ALoop_0, IHa2; assumption.
 Qed.
+
+Fixpoint append (r1 r2 : relir) : relir :=
+  match r1 with
+  | RMove n r1' => RMove n (append r1' r2)
+  | RAdd n off r1' => RAdd n off (append r1' r2)
+  | ROutput off r1' => ROutput off (append r1' r2)
+  | RInput off r1' => RInput off (append r1' r2)
+  | RLoop body r1' => RLoop body (append r1' r2)
+  | REnd => r2
+  end.
+
+Theorem append_end_l : forall r,
+  append REnd r = r.
+Proof. reflexivity. Qed.
+
+Theorem append_end_r : forall r,
+  append r REnd = r.
+Proof.
+  induction r; cbn;
+  try rewrite IHr; try rewrite IHr2; reflexivity. Qed.
+
+Theorem execute_append : forall r1 r2 v v' v'',
+  execute r1 v v' ->
+  execute r2 v' v'' ->
+  execute (append r1 r2) v v''.
+Proof.
+  induction r1; intros; cbn;
+  try (inversion H; subst; econstructor; [eassumption | eapply IHr1; eassumption]).
+  - dependent induction H.
+    + eapply E_RLoop. assumption. eassumption. now apply IHexecute2.
+    + eapply E_RLoop_0. assumption. eapply IHr1_2; eassumption.
+  - inversion H; subst. admit.
+Admitted.
+
+Theorem execute_append_split : forall r1 r2 v v'',
+  execute (append r1 r2) v v'' ->
+  exists v', execute r1 v v' /\ execute r2 v' v''.
+Proof.
+  induction r1; cbn; intros.
+  - inversion H; subst. apply IHr1 in H5 as [v'1 []].
+    exists v'1. split; [eapply E_RMove |]; eassumption.
+  - inversion H; subst. apply IHr1 in H6 as [v'1 []].
+    exists v'1. split; [eapply E_RAdd |]; eassumption.
+  - inversion H; subst. apply IHr1 in H5 as [v'1 []].
+    exists v'1. split; [eapply E_ROutput |]; eassumption.
+  - inversion H; subst. apply IHr1 in H5 as [v'1 []].
+    exists v'1. split; [eapply E_RInput |]; eassumption.
+  - admit.
+  - exists v. split. apply E_REnd. apply RelVM.eq_refl. assumption.
+Admitted.
